coq-osiris/theories/program_logic/pure/expr_rules.v
@@ -1380,7 +1380,7 @@ Proof.
   apply pure_wp_handle.
   apply (pure_wp_mono _ Heval); [ | intros _ [] ].
   intros ? (? & -> & ->).
-  unfold continue. simpl.
+  unfold continue. simpl_wrap_eval_branches.
   apply (pure_wp_mono _ Hmatch); eauto.
 Qed.
 
@@ -1394,7 +1394,7 @@ Proof.
   apply pure_wp_handle.
   apply (pure_wp_mono _ Heval). 2: intros _ [].
   intros ? (a & -> & Ha).
-  unfold continue. simpl.
+  unfold continue. simpl_wrap_eval_branches.
   apply (pure_wp_mono _ (Hmatch _ Ha)); eauto.
 Qed.
 
@@ -1410,10 +1410,10 @@ Proof.
   apply pure_wp_handle.
   apply (pure_wp_mono _ He).
   - intros _v (a & -> & Ha).
-    unfold continue. simpl.
+    unfold continue. simpl_wrap_eval_branches.
     by apply Hφ'.
   - intros ex Hex.
-    unfold discontinue. simpl.
+    unfold discontinue. simpl_wrap_eval_branches.
     by apply Hζ.
 Qed.
 
